

①

Beta Function.

$$\beta(m, n) = \int_0^1 x^{m-1} (1-x)^{n-1} dx \quad \text{--- ①}$$

Also  $\beta(m, n) = \beta(n, m)$  [Symmetry]

Now put  $x = \frac{t}{1+t}$  in eq. ①.

When  $x = 0$   
 $t = 0$   
 $\Rightarrow x(1+t) = t \Rightarrow x + xt = t \Rightarrow x = t(1-x)$   
 $\Rightarrow \boxed{t = \frac{x}{1-x}}$

When  $x = 1 \Rightarrow t = \infty$

Also  $dx = \frac{(1+t) \cdot 1 - t(1)}{(1+t)^2} dt = \frac{1+t-t}{(1+t)^2} dt$

$$\Rightarrow dx = \frac{dt}{(1+t)^2}$$

Now from eq. ① we have.

$$\beta(m, n) = \int_0^{\infty} \left( \frac{t}{1+t} \right)^{m-1} \left( 1 - \frac{t}{1+t} \right)^{n-1} \frac{dt}{(1+t)^2}$$

$$\beta(m, n) = \int_0^{\infty} \frac{t^{m-1}}{(1+t)^{m-1}} \left( \frac{1+t-t}{1+t} \right)^{n-1} \frac{dt}{(1+t)^2}$$

$$= \int_0^{\infty} \frac{t^{m-1}}{(1+t)^{m-1}} \cdot \frac{1}{(1+t)^{n-1}} \cdot \frac{dt}{(1+t)^2}$$

$$= \int_0^{\infty} \frac{t^{m-1} dt}{(1+t)^{m-1+n-1+2}} = \int_0^{\infty} \frac{t^{m-1}}{(1+t)^{m+n}} dt$$

$$\therefore \beta(m, n) = \int_0^{\infty} \frac{t^{m+1}}{(1+t)^{m+n}} dt.$$

Also As  $\beta$ -function is symmetrical

$$\therefore \beta(m, n) = \int_0^{\infty} \frac{t^{n+1}}{(1+t)^{m+n}} dt.$$

Another form of  $\beta$ -function.

$$\beta(m, n) = \int_0^1 x^{m+1} (1-x)^{n+1} dx.$$

$$\text{Put } x = \sin^2 \theta$$

$$\Rightarrow dx = 2 \sin \theta \cos \theta d\theta.$$

$$\text{Also when } x=0 \Rightarrow \sin^2 \theta = 0 \Rightarrow \theta=0$$

$$\text{when } x=1 \Rightarrow \sin^2 \theta = 1 \Rightarrow \theta = \pi/2.$$

$$\begin{aligned} \therefore \beta(m, n) &= \int_0^{\pi/2} (\sin^2 \theta)^{m+1} (1 - \sin^2 \theta)^{n+1} 2 \sin \theta \cos \theta d\theta \\ &= \int_0^{\pi/2} (\sin \theta)^{2m+2} (\cos \theta)^{2n+2} \cdot 2 \sin \theta \cos \theta d\theta \end{aligned}$$

$$\therefore \beta(m, n) = 2 \int_0^{\pi/2} (\sin \theta)^{2m+1} (\cos \theta)^{2n+1} d\theta$$

$$\beta(m, n) = 2 \int_0^{\pi/2} \sin^{2m+1} \theta \cos^{2n+1} \theta d\theta$$

$$\beta(m, n) = \int_0^{\infty} \frac{t^{m-1}}{(1+t)^{m+n}} dt \quad \text{--- (2)}$$

$$= \int_0^1 \frac{t^{m-1}}{(1+t)^{m+n}} dt + \int_1^{\infty} \frac{t^{m-1}}{(1+t)^{m+n}} dt \quad \text{---}$$

Let  $t = \frac{1}{z}$  in second integral only.

when  $t=1$ ,  $z=1$  Also  $dt = -\frac{1}{z^2} dz$   
 when  $t=\infty$ ,  $z=0$

$$\therefore \int_1^{\infty} \frac{t^{m-1}}{(1+t)^{m+n}} dt = \int_1^0 \frac{\left(\frac{1}{z}\right)^{m-1}}{\left(1+\frac{1}{z}\right)^{m+n}} \left(-\frac{1}{z^2}\right) dz$$

$$= \int_1^0 \frac{1}{z^{m-1}} \times \frac{1}{\left(\frac{z+1}{z}\right)^{m+n}} \left(-\frac{1}{z^2}\right) dz$$

$$= - \int_1^0 \frac{1}{z^{m-1+2}} \cdot \frac{z^{m+n}}{(1+z)^{m+n}} dz$$

$$= \int_0^1 \frac{z^{m+n-m-1}}{(1+z)^{m+n}} dz \quad \left( \because \int_a^b f(x) dx = - \int_b^a f(x) dx \right)$$

$$= \int_0^1 \frac{z^{n-1}}{(1+z)^{m+n}} dz$$

$$= \int_0^1 \frac{t^{n-1}}{(1+t)^{m+n}} dt \quad \text{--- (3)}$$

Using (3) in (2)

$$\beta(m, n) = \int_0^1 \frac{t^{m-1}}{(1+t)^{m+n}} dt + \int_0^1 \frac{t^{n-1}}{(1+t)^{m+n}} dt$$

$$\therefore \beta(m, n) = \int_0^1 \frac{t^{m-1} + t^{n-1}}{(1+t)^{m+n}} dt$$

So we've

$$(1) \quad \beta(m, n) = \int_0^1 x^{m-1} (1-x)^{n-1} dx$$

$$(2) \quad = \int_0^1 x^{n-1} (1-x)^{m-1} dx.$$

$$(3) \quad = 2 \int_0^{\pi/2} \sin^{2m-1} \theta \cos^{2n-1} \theta d\theta.$$

$$(4) \quad = \int_0^{\infty} \frac{x^{m-1}}{(1+x)^{m+n}} dx = \int_0^{\infty} \frac{x^{n-1}}{(1+x)^{m+n}} dx.$$

$$(5) \quad = \int_0^1 \frac{x^{m-1} + x^{n-1}}{(1+x)^{m+n}} dx.$$